src/impl/TLS13.Impl.Server.fsti
@@ -407,6 +407,46 @@ fn process_send_encrypted_extensions_serialized
                   network_out_bytes
                   app_out_bytes)
 
+fn process_send_server_finished_serialized
+  (s:server)
+  (network_out:array U8.t)
+  (network_out_len:SZ.t)
+  (app_out:array U8.t)
+  (app_out_len:SZ.t)
+  requires connection_exactly s 'st0 **
+           pts_to network_out 'old_network_out **
+           pts_to app_out 'old_app_out **
+           pure (B.length 'old_network_out == SZ.v network_out_len /\
+                 B.length 'old_app_out == SZ.v app_out_len /\
+                 SZ.v network_out_len == 58 /\
+                 ST.server_end_to_end_invariant 'st0 /\
+                 'st0.CS.cs_model.CS.model_control ==
+                   CS.ControlHandshaking CS.HsServerEncryptedFlightSent /\
+                 'st0.CS.cs_model.CS.model_config.CS.config_role ==
+                   CS.ServerEndpoint /\
+                 'st0.CS.cs_model.CS.model_handshake.CS.hs_certificate_verify_verified /\
+                 Some?
+                   'st0.CS.cs_model.CS.model_handshake.CS.hs_keys.CS.ks_server_handshake_traffic /\
+                 U64.fits
+                   ('st0.CS.cs_model.CS.model_record.CS.record_write.R.seq + 1) /\
+                 B.length 'st0.CS.cs_model.CS.model_handshake.CS.hs_transcript + 36 <=
+                   Bounds.max_transcript_len)
+  returns resp:ST.server_response
+  ensures exists* st1 network_out_bytes app_out_bytes.
+          connection_exactly s st1 **
+          pts_to network_out network_out_bytes **
+          pts_to app_out app_out_bytes **
+          pure (B.length network_out_bytes == SZ.v network_out_len /\
+                B.length app_out_bytes == SZ.v app_out_len /\
+                ST.server_local_event_end_to_end_correct
+                  'st0
+                  st1
+                  resp
+                  ST.LocalSendServerFinished
+                  B.empty
+                  network_out_bytes
+                  app_out_bytes)
+
 fn process_derive_shared_secret
   (s:server)
   (shared_src:array U8.t)
